src/coqutil/Map/SeparationMemory.v
@@ -1,0 +1,125 @@
+From Coq Require Import List BinInt ZArith Lia Init.Byte.
+From coqutil Require Import Word.Interface Map.Interface Map.OfListWord Memory SeparationLogic Lift1Prop LittleEndianList.
+From coqutil Require Import Word.Properties Map.Properties Tactics Macros.symmetry.
+
+Local Coercion word.unsigned : word.rep >-> Z.
+
+Section SeparationMap.
+  Local Open Scope sep_scope.
+  Local Coercion Z.of_nat : nat >-> Z.
+  Local Infix "$+" := map.putmany (at level 70).
+
+  Context {width : Z} {word : Word.Interface.word width} {word_ok : word.ok word}.
+  Context [value] [map : map.map word value] {ok : map.ok map}.
+  Add Ring __wring: (@word.ring_theory width word word_ok).
+
+  (** * [++] *)
+
+  Lemma sep_eq_of_list_word_at_app (a : word) (xs ys : list value)
+    lxs (Hlxs : Z.of_nat (length xs) = lxs) (Htotal : length xs + length ys <= 2^width)
+    : Lift1Prop.iff1 (eq ((xs ++ ys)$@a))
+      (sep (eq (xs$@a)) (eq (ys$@(word.add a (word.of_Z lxs))))).
+  Proof.
+    etransitivity.
+    2: eapply sep_comm.
+    etransitivity.
+    2: eapply sep_eq_putmany, map.adjacent_arrays_disjoint_n; trivial.
+    erewrite map.of_list_word_at_app_n by eauto; reflexivity.
+  Qed.
+
+  Lemma list_word_at_app_of_adjacent_eq (a b : word) (xs ys : list value)
+    (Hl: word.unsigned (word.sub b a) = Z.of_nat (length xs))
+    (Htotal : length xs + length ys <= 2^width)
+    : Lift1Prop.iff1 (eq(xs$@a)*eq(ys$@b)) (eq((xs++ys)$@a)).
+  Proof.
+    etransitivity.
+    2:symmetry; eapply sep_eq_of_list_word_at_app; trivial.
+    do 3 Morphisms.f_equiv. rewrite <-Hl, word.of_Z_unsigned. ring.
+  Qed.
+End SeparationMap.
+
+Section SeparationMemory.
+  Local Open Scope sep_scope.
+  Local Coercion Z.of_nat : nat >-> Z.
+  Local Infix "$+" := map.putmany (at level 70).
+
+  Context {width : Z} {word : Word.Interface.word width} {word_ok : word.ok word}.
+  Context [mem : map.map word byte] {ok : map.ok mem}.
+  Add Ring __wring: (@word.ring_theory width word word_ok).
+
+  (** * Load *)
+
+  Lemma load_bytes_of_sep bs a n R (m : mem) (Hsep: m =* bs$@a*R)
+    (Hl : length bs = n%nat) (Hlw : Z.of_nat n < 2 ^ width) :
+    load_bytes m a n = Some bs.
+  Proof.
+    apply sep_comm in Hsep.
+    case Hsep as (mR&mbs&[-> disj]&?&?); cbv [sepclause_of_map] in *; subst mbs.
+    auto using load_bytes_of_putmany_bytes_at.
+  Qed.
+
+  Lemma load_Z_of_sep bs a n R (m : mem) (Hsep: m =* bs$@a*R)
+    (Hl : length bs = n%nat) (Hlw : Z.of_nat n < 2 ^ width) : 
+    load_Z m a n = Some (LittleEndianList.le_combine bs).
+  Proof. cbv [load_Z]. erewrite load_bytes_of_sep; eauto. Qed.
+
+  Lemma uncurried_load_Z_of_sep bs a n R (m : mem)
+    (H : m =* bs$@a * R /\ length bs = n%nat /\ Z.of_nat n < 2 ^ width) :
+    load_Z m a n = Some (LittleEndianList.le_combine bs).
+  Proof. eapply load_Z_of_sep; eapply H. Qed.
+
+  Lemma uncurried_load_Z_of_sep_Z bs a n R (m : mem)
+    (H : m =* bs$@a * R /\ Z.of_nat (length bs) = n%nat /\ n < 2 ^ width) :
+    load_Z m a (Z.to_nat n) = Some (LittleEndianList.le_combine bs).
+  Proof. eapply load_Z_of_sep; try eapply H; lia. Qed.
+
+  Lemma uncurried_load_Z_of_sep_word bs a (n : word) R (m : mem)
+    (H : m =* bs$@a * R /\ Z.of_nat (length bs) = n) :
+    load_Z m a (Z.to_nat (word.unsigned n)) = Some (LittleEndianList.le_combine bs).
+  Proof.
+    case (word.unsigned_range n) as [].
+    eapply uncurried_load_Z_of_sep_Z; intuition eauto.
+  Qed.
+
+  (** * Store *)
+
+  Lemma uncurried_unchecked_store_bytes_of_sep (a: word) (n: nat) (_bs bs: list byte)
+    (R: mem -> Prop) (m: mem) (H : m =* _bs$@a * R /\ length _bs = n /\ length bs = n) :
+    Memory.unchecked_store_bytes m a bs =* bs$@a * R.
+  Proof.
+    cbv [unchecked_store_bytes].
+    case H as ((mR&mbs&[->disj]&?&?)%sep_comm &_bs_l&bs_l).
+    cbv [sepclause_of_map] in *; subst mbs.
+    eexists _, _; ssplit; eauto; [].
+    rewrite <-map.putmany_assoc.
+    eassert (_bs$@a $+ bs$@a = bs$@a) as ->.
+    { apply map.map_ext; intros k; rewrite !map.get_putmany_dec, ?map.get_of_list_word_at.
+      destruct nth_error eqn:?; trivial; []; rewrite ?nth_error_None in *; lia. }
+    apply map.split_comm; split; trivial; [].
+    apply map.disjoint_comm in disj; apply map.disjoint_comm.
+    eapply map.sub_domain_disjoint; [exact disj|].
+    cbv [map.sub_domain]; intros k v; rewrite ?map.get_of_list_word_at.
+    intros ?%List.nth_error_Some_bound_index.
+    destruct nth_error eqn:X; eauto; []; exfalso.
+    eapply nth_error_None in X; lia.
+  Qed.
+
+  Lemma uncurried_store_bytes_of_sep (a: word) (n: nat) (_bs bs: list byte)
+    (R: mem -> Prop) (m: mem) (H : m =* _bs$@a * R /\ length _bs = n /\ length bs = n /\ n < 2^width) :
+    exists m', Memory.store_bytes m a bs = Some m' /\ m' =* bs$@a * R.
+  Proof.
+    cbv [store_bytes]; intuition idtac.
+    erewrite load_bytes_of_sep; eauto; try lia.
+    eexists; ssplit; eauto.
+    eapply uncurried_unchecked_store_bytes_of_sep; eauto.
+  Qed.
+
+  Lemma uncurried_store_Z_of_sep (a: word) (n: nat) (_bs : list byte) (z : Z)
+    (R: mem -> Prop) (m: mem) (H : m =* _bs$@a * R /\ length _bs = n /\ n < 2^width) :
+    exists m', Memory.store_Z m a n z = Some m' /\ m' =* (le_split n z)$@a * R.
+  Proof.
+    cbv [Memory.store_Z].
+    eapply uncurried_store_bytes_of_sep; intuition eauto with nocore;
+    rewrite ?length_le_split; lia.
+  Qed.
+End SeparationMemory.
